Prove postcondition for RD operations
The Write specifications are far too complicated at the moment. There
are a large number of cases, and perhaps handling them separately rather
than trying to express specifications that cover many possibilities,
would lead to overall shorter proofs with more automation and small,
focused lemmas.

The fact that crash invariants have to re-prove the postcondition is
also really painful, when it would be easy to prove the spec satisfies
postcond => crashinv.

Shallow/ReplicatedDisk.v
@@ -200,6 +200,442 @@ Module RD.
 
   Hint Constructors D.step.
 
+  Lemma abstraction_set_d0 : forall state d a b,
+      TD.get_disk d0 state = Some d ->
+      abstraction (TD.set_disk d0 state (upd d a b)) =
+      D.SDisk (upd (D.sdisk (abstraction state)) a b).
+  Proof.
+    intros.
+    destruct state; simpl in *.
+    destruct disk0; simpl; congruence.
+  Qed.
+
+  Definition invariant_except (state:TD.State) a b :=
+    match state with
+    | TD.Disks (Some d_0) (Some d_1) _ =>
+      (exists b0, d_1 a = Some b0) /\
+      d_0 = upd d_1 a b
+    | TD.Disks (Some d_0) None _ =>
+      d_0 a = Some b
+    | TD.Disks None (Some _) _ => False
+    | _ => True
+    end.
+
+  Lemma invariant_except_upd_d0 : forall state d a b0 b,
+      invariant state ->
+      TD.disk0 state = Some d ->
+      d a = Some b0 ->
+      invariant_except (TD.set_disk d0 state (upd d a b)) a b.
+  Proof.
+    unfold invariant, invariant_except; intros.
+    destruct matches in *|- ;
+      simpl in *;
+      intuition;
+      try congruence.
+    match goal with
+    | [ H: Some _ = Some _ |- _ ] =>
+      inversion H; subst; clear H
+    end; eauto.
+    autorewrite with upd; auto.
+  Qed.
+
+  Hint Resolve invariant_except_upd_d0.
+
+  Lemma abstraction_is_some_disk : forall state,
+      {exists d, TD.get_disk d0 state = Some d /\
+            abstraction state = D.SDisk d} +
+      {exists d, TD.get_disk d1 state = Some d /\
+            abstraction state = D.SDisk d /\
+            TD.get_disk d0 state = None}.
+  Proof.
+    intros.
+    destruct state; simpl.
+    destruct matches;
+      eauto.
+    exfalso; repeat deex; intuition congruence.
+  Qed.
+
+  Ltac case_abstraction :=
+    match goal with
+    | [ H: context[D.sdisk (abstraction ?state)] |- _ ] =>
+      destruct (abstraction_is_some_disk state);
+      repeat deex;
+      match goal with
+      | [ H: abstraction _ = _ |- _ ] =>
+        rewrite H in *; cbn [D.sdisk] in *
+      end
+    end.
+
+  Lemma invariant_stability : forall state state',
+      invariant state ->
+      TD.bg_step state state' ->
+      abstraction state = abstraction state' /\
+      invariant state'.
+  Proof.
+    intros.
+    intuition eauto.
+    symmetry; auto.
+  Qed.
+
+  Ltac inv_stable :=
+    match goal with
+    | [ H: invariant ?state,
+           H': TD.bg_step ?state ?state' |- _ ] =>
+      pose proof (invariant_stability H H');
+      clear H H';
+      safe_intuition;
+      replace (abstraction state) in *
+    end.
+
+  Theorem TDWrite0_inbounds_ok : forall a b,
+      prog_spec
+        (fun b0 (state:TD.State) =>
+           {|
+             pre := invariant state /\
+                    D.sdisk (abstraction state) a = Some b0;
+             post :=
+               fun r state' =>
+                 (abstraction state' = D.SDisk (upd (D.sdisk (abstraction state)) a b) /\
+                  invariant_except state' a b) \/
+                 (abstraction state' = abstraction state /\
+                  first_disk_failed state');
+             crash :=
+               fun state' =>
+                 (abstraction state' = abstraction state /\
+                  invariant state') \/
+                 (abstraction state' = D.SDisk (upd (D.sdisk (abstraction state)) a b) /\
+                  (* this should be a recoverable property *)
+                  invariant_except state' a b)
+           |})
+        (Prim (TD.Write d0 a b))
+        TD.step.
+  Proof.
+    unfold prog_spec; cbn [pre post crash]; intuition.
+    inv_exec; eauto.
+    - TD.inv_step.
+      subst_var.
+      inv_stable.
+      case_abstraction;
+        repeat simpl_match;
+        eauto.
+      rewrite abstraction_set_d0 by auto.
+      replace (abstraction x); cbn [D.sdisk]; eauto.
+    - TD.inv_step; subst_var.
+      inv_stable.
+      case_abstraction;
+        repeat simpl_match;
+        eauto.
+      rewrite abstraction_set_d0 by auto.
+      replace (abstraction x); cbn [D.sdisk]; eauto.
+  Qed.
+
+  Lemma invariant_both_disks : forall state d_0 d_1,
+      invariant state ->
+      TD.get_disk d0 state = Some d_0 ->
+      TD.get_disk d1 state = Some d_1 ->
+      d_0 = d_1.
+  Proof.
+    unfold invariant; intros; destruct matches in *;
+      simpl in *;
+      congruence.
+  Qed.
+
+  Theorem TDWrite_oob_ok : forall i a b,
+      prog_spec
+        (fun (_:unit) (state:TD.State) =>
+           {|
+             pre := invariant state /\
+                    D.sdisk (abstraction state) a = None;
+             post :=
+               fun r state' =>
+                 abstraction state' = abstraction state /\
+                 invariant state';
+             crash :=
+               fun state' =>
+                 abstraction state' = abstraction state /\
+                 invariant state'
+           |})
+        (Prim (TD.Write i a b))
+        TD.step.
+  Proof.
+    unfold prog_spec; cbn [pre post crash]; intuition.
+    inv_exec; eauto.
+    - TD.inv_step.
+      subst_var.
+      inv_stable.
+      destruct i; case_abstraction;
+        repeat simpl_match;
+        eauto.
+      destruct (TD.get_disk d1 x) eqn:?; eauto.
+      pose proof (invariant_both_disks _ H0 ltac:(eauto) ltac:(eauto));
+        subst.
+      simpl_match; eauto.
+    - TD.inv_step.
+      subst_var.
+      inv_stable.
+      destruct i; case_abstraction;
+        repeat simpl_match;
+        eauto.
+      destruct (TD.get_disk d1 x) eqn:?; eauto.
+      pose proof (invariant_both_disks _ H0 ltac:(eauto) ltac:(eauto));
+        subst.
+      simpl_match; eauto.
+  Qed.
+
+  Theorem invariant_except_step : forall state a b state',
+      invariant_except state a b ->
+      TD.bg_step state state' ->
+      (invariant_except state' a b \/
+       invariant state').
+  Proof.
+    inversion 2; subst; simpl in *; eauto.
+  Qed.
+
+  Hint Resolve invariant_except_step.
+
+  Lemma invariant_except_to_invariant : forall state d a b,
+      invariant_except state a b ->
+      TD.get_disk d1 state = Some d ->
+      invariant (TD.set_disk d1 state (upd d a b)).
+  Proof.
+    unfold invariant_except; intros.
+    destruct state; simpl in *; subst; auto.
+    destruct matches; safe_intuition; eauto.
+  Qed.
+
+  Hint Resolve invariant_except_to_invariant.
+
+  Ltac cleanup :=
+    repeat match goal with
+           | _ => progress safe_intuition
+           | _ => simpl_match
+           | _ => deex
+           | _ => progress subst
+           | _ => progress simpl in *
+           | _ => contradiction
+           | [ H: None = Some _ \/ None = Some _ |- _ ] =>
+             exfalso; destruct H; congruence
+           | [ H: Some _ = Some _ |- _ ] =>
+             inversion H; subst; clear H
+           | _ => progress eauto
+           | _ => congruence
+           end.
+
+  Lemma invariant_except_after_step : forall state state' a b,
+      invariant_except state a b ->
+      TD.bg_step state state' ->
+      (* d0 survived *)
+      (exists d, TD.get_disk d0 state' = Some d /\
+            abstraction state' = D.SDisk d /\
+            d a = Some b /\
+            invariant_except state' a b) \/
+      (* only d1 survived *)
+      (exists b0 d, TD.get_disk d1 state' = Some d /\
+               abstraction state' = D.SDisk d /\
+               d a = Some b0 /\
+               TD.get_disk d0 state' = None).
+  Proof.
+    inversion 2; cleanup; eauto 10 using upd_eq.
+    unfold invariant_except in H; destruct matches in *;
+      cleanup;
+      eauto 10 using upd_eq.
+  Qed.
+
+  Lemma invariant_except_set_d1 : forall state d' a b,
+      invariant_except state a b ->
+      abstraction (TD.set_disk d1 state d') = abstraction state.
+  Proof.
+    intros.
+    unfold invariant_except, abstraction in *;
+      destruct matches in *;
+      simpl in *;
+      try match goal with
+          | [ H: TD.Disks _ _ _ = TD.Disks _ _ _ |- _ ] =>
+            inversion H; subst; clear H
+          end;
+      cleanup.
+  Qed.
+
+  Lemma invariant_except_known_d0 : forall state d a b,
+      TD.get_disk d0 state = Some d ->
+      invariant_except state a b ->
+      (TD.get_disk d1 state = None \/
+       exists b0 d', TD.get_disk d1 state = Some d' /\
+             d' a = Some b0 /\
+             d = upd d' a b).
+  Proof.
+    unfold invariant_except; intros.
+    destruct matches in *; cleanup.
+    eauto 10.
+  Qed.
+
+  Lemma bg_step_invert : forall state d_0 d_1 pf,
+      TD.bg_step state (TD.Disks (Some d_0) (Some d_1) pf) ->
+      state = TD.Disks (Some d_0) (Some d_1) pf.
+  Proof.
+    intros.
+    inversion H; subst; eauto.
+  Qed.
+
+  Lemma invariant_except_no_d1 : forall state a b,
+      invariant_except state a b ->
+      TD.disk1 state = None ->
+      invariant state.
+  Proof.
+    unfold invariant_except; intros;
+      destruct matches in *;
+      cleanup.
+  Qed.
+
+  Hint Resolve invariant_except_no_d1.
+
+  Theorem TDWrite1_inbounds_d0_ok : forall a b,
+      prog_spec
+        (fun (_:unit) (state:TD.State) =>
+           {|
+             pre := invariant_except state a b;
+             post :=
+               fun r state' =>
+                 abstraction state' = abstraction state /\
+                 invariant state';
+             crash :=
+               fun state' =>
+                 (abstraction state' = abstraction state /\
+                  invariant_except state' a b) \/
+                 (abstraction state' = abstraction state /\
+                  invariant state')
+                 (* missing crash case: we might actually lose the first disk
+                 and thus undo the pending write, but this isn't a possible
+                 crash state; the fix is either to allow a bg_step right after
+                 crash, to add a new crash state after a disk possibly fails but
+                 before the write runs *)
+                 (* (exists d, TD.disk1 state = Some d /\
+                       abstraction state' = D.SDisk d) *);
+           |})
+        (Prim (TD.Write d1 a b))
+        TD.step.
+  Proof.
+    unfold prog_spec; cbn [pre post crash]; intuition.
+    inv_exec; eauto.
+    - TD.inv_step.
+      subst_var.
+      destruct (invariant_except_after_step _ _ H H0);
+        repeat deex.
+      destruct (invariant_except_known_d0 _ _ _ H1 H4);
+        cleanup.
+      inversion H0; cleanup; intuition eauto.
+
+      destruct matches; simpl in *; destruct matches in *;
+        cleanup;
+        intuition eauto.
+      eapply bg_step_invert in H0; subst; simpl; eauto.
+
+      destruct matches; simpl in *; destruct matches in *;
+        cleanup;
+        intuition eauto.
+      destruct disk0, disk1; cleanup.
+      inversion H0; subst; cleanup.
+    - right.
+      TD.inv_step.
+      subst_var.
+      destruct (invariant_except_after_step _ _ H H0);
+        repeat deex.
+      destruct (invariant_except_known_d0 _ _ _ H1 H4);
+        cleanup.
+      inversion H0; cleanup; intuition eauto.
+
+      destruct matches; simpl in *; destruct matches in *;
+        cleanup;
+        intuition eauto.
+      eapply bg_step_invert in H0; subst; simpl; eauto.
+
+      destruct matches; simpl in *; destruct matches in *;
+        cleanup;
+        intuition eauto.
+      destruct disk0, disk1; cleanup.
+      inversion H0; subst; cleanup.
+  Qed.
+
+  Theorem TDWrite1_inbounds_no_d0_ok : forall a b,
+      prog_spec
+        (fun b0 (state:TD.State) =>
+           {|
+             pre := invariant state /\
+                    first_disk_failed state /\
+                    D.sdisk (abstraction state) a = Some b0;
+             post :=
+               fun r state' =>
+                 abstraction state' = D.SDisk (upd (D.sdisk (abstraction state)) a b) /\
+                 invariant state';
+             crash :=
+               fun state' =>
+                 (abstraction state' = abstraction state /\
+                  invariant state') \/
+                 (abstraction state' = D.SDisk (upd (D.sdisk (abstraction state)) a b) /\
+                 invariant state');
+           |})
+        (Prim (TD.Write d1 a b))
+        TD.step.
+  Proof.
+    unfold prog_spec; cbn [pre post crash]; intuition.
+    inv_exec; eauto.
+    - TD.inv_step.
+      subst_var.
+      eapply bg_step_after_fail in H1; eauto; subst.
+      case_abstraction;
+        unfold first_disk_failed in *;
+        cleanup.
+      destruct matches in *;
+        cleanup;
+        destruct matches in *.
+    - TD.inv_step.
+      subst_var.
+      eapply bg_step_after_fail in H1; eauto; subst.
+      case_abstraction;
+        unfold first_disk_failed in *;
+        cleanup.
+      destruct matches in *;
+        cleanup;
+        destruct matches in *.
+  Qed.
+
+  Lemma step_write_inbounds : forall state a b0 b,
+      D.sdisk state a = Some b0 ->
+      D.step (D.Write a b) state tt
+             (D.SDisk (upd (D.sdisk state) a b)).
+  Proof.
+    intros.
+    pose proof (D.step_write a b state); simpl in *.
+    simpl_match.
+    auto.
+  Qed.
+
+  Hint Resolve step_write_inbounds.
+
+  Lemma invariant_first_disk_failed : forall state,
+      first_disk_failed state ->
+      invariant state.
+  Proof.
+    unfold first_disk_failed, invariant;
+      intros;
+      destruct matches in *;
+      cleanup.
+  Qed.
+
+  Hint Resolve invariant_first_disk_failed.
+
+  Lemma step_write_oob : forall state a b,
+      D.sdisk state a = None ->
+      D.step (D.Write a b) state tt state.
+  Proof.
+    intros.
+    pose proof (D.step_write a b state); simpl in *.
+    simpl_match.
+    destruct state; eauto.
+  Qed.
+
+  Hint Resolve step_write_oob.
+
   Theorem RD_ok : interpretation
                     op_impl
                     TD.step D.step
@@ -231,9 +667,44 @@ Module RD.
                end.
         intuition eauto.
       + inv_exec.
-        (* TODO: prove and use Write specs *)
-        admit.
-    - (* also need crash proofs *)
+        destruct (D.sdisk (abstraction state) a) eqn:?.
+        eapply TDWrite0_inbounds_ok in H6; eauto;
+          cbn [pre post crash] in *;
+          cleanup.
+        hyp_intuition.
+        inv_exec.
+        eapply TDWrite1_inbounds_d0_ok in H7; eauto;
+          cbn [pre post crash] in *;
+          cleanup.
+        repeat match goal with
+               | [ H: abstraction _ = _ |- _ ] =>
+                 rewrite H
+               end.
+        intuition eauto.
+
+        inv_exec.
+        eapply TDWrite1_inbounds_no_d0_ok in H7; eauto;
+          cbn [pre post crash] in *;
+          cleanup;
+          repeat match goal with
+                 | [ H: abstraction _ = _ |- _ ] =>
+                   rewrite H
+                 end;
+          intuition eauto.
+
+        eapply TDWrite_oob_ok in H6; eauto;
+          cbn [pre post crash] in *;
+          cleanup.
+        inv_exec.
+        eapply TDWrite_oob_ok in H7; eauto;
+          cbn [pre post crash] in *;
+          cleanup;
+          repeat match goal with
+                 | [ H: abstraction _ = _ |- _ ] =>
+                   rewrite H
+                 end;
+          intuition eauto.
+    - (* also need a crash proof *)
   Abort.
 
 End RD.
